Vsa.lean
@@ -143,6 +143,7 @@ import Vsa.Sim.ExecSimCommon
 import Vsa.Sim.Exec_stmtSites
 import Vsa.Sim.ExecBrkCont
 import Vsa.Sim.ExecExprRet
+import Vsa.Sim.ExecRecCommon
 import Vsa.Sim.BlockLogic
 import Vsa.Sim.ReprSurvival
 import Vsa.Sim.ReprCopy
